prove parse sort-of left inverts print

examples/lpr_checker/parsingScript.sml
@@ -12,42 +12,201 @@ val _ = new_theory "parsing";
 val blanks_def = Define`
   blanks (c:char) ⇔ c = #" " ∨ c = #"\n" ∨ c = #"\t"`
 
+(* DIMACS parser *)
+
 (*
   A clause line must end with 0, cannot contain 0s elsewhere, and is within the var bound
 *)
-val parse_clause_def = Define`
-  (parse_clause maxvar [] (acc:cclause) = NONE) ∧
-  (parse_clause maxvar [c] acc =
+
+(* TODO: mlint fromString should return NONE on empty *)
+val parse_clause_aux_def = Define`
+  (parse_clause_aux maxvar [] (acc:cclause) = NONE) ∧
+  (parse_clause_aux maxvar [c] acc =
     if c = (strlit "0") then SOME acc
     else NONE) ∧
-  (parse_clause maxvar (x::xs) acc =
+  (parse_clause_aux maxvar (x::xs) acc =
     case mlint$fromString x of
       NONE => NONE
     | SOME l =>
     if l = 0 ∨ Num (ABS l) > maxvar then NONE
-    else parse_clause maxvar xs (l::acc)
+    else parse_clause_aux maxvar xs (l::acc)
   )`
 
-Theorem parse_clause_wf_clause:
+val parse_clause_def = Define`
+  parse_clause maxvar xs =
+  case parse_clause_aux maxvar xs [] of
+    NONE => NONE
+  | SOME ls => SOME (REVERSE ls)`
+
+Theorem parse_clause_aux_wf_clause:
   ∀mv ls acc acc'.
   wf_clause acc ∧
-  parse_clause mv ls acc = SOME acc' ⇒
+  parse_clause_aux mv ls acc = SOME acc' ⇒
   wf_clause acc'
 Proof
-  ho_match_mp_tac (fetch "-" "parse_clause_ind")>>
-  rw[parse_clause_def]>>fs[wf_clause_def]>>
+  ho_match_mp_tac (fetch "-" "parse_clause_aux_ind")>>
+  rw[parse_clause_aux_def]>>fs[wf_clause_def]>>
+  every_case_tac>>fs[]
+QED
+
+Theorem parse_clause_wf_clause:
+  parse_clause mv ls = SOME ls' ⇒
+  wf_clause ls'
+Proof
+  simp[parse_clause_def]>>every_case_tac>>rw[]>>
+  imp_res_tac parse_clause_aux_wf_clause>>
+  fs[wf_clause_def]
+QED
+
+Theorem parse_clause_aux_bound:
+  ∀mv ls acc acc'.
+  EVERY (λi. Num (ABS i) <= mv) acc ∧
+  parse_clause_aux mv ls acc = SOME acc' ⇒
+  EVERY (λi. Num (ABS i) <= mv) acc'
+Proof
+  ho_match_mp_tac (fetch "-" "parse_clause_aux_ind")>>
+  rw[parse_clause_aux_def]>>
   every_case_tac>>fs[]
 QED
 
 Theorem parse_clause_bound:
-  ∀mv ls acc acc'.
-  EVERY (λi. Num (ABS i) <= mv) acc ∧
-  parse_clause mv ls acc = SOME acc' ⇒
-  EVERY (λi. Num (ABS i) <= mv) acc'
+  parse_clause mv ls = SOME ls' ⇒
+  EVERY (λi. Num (ABS i) <= mv) ls'
 Proof
-  ho_match_mp_tac (fetch "-" "parse_clause_ind")>>
-  rw[parse_clause_def]>>fs[wf_clause_def]>>
-  every_case_tac>>fs[]
+  simp[parse_clause_def]>>every_case_tac>>rw[]>>
+  imp_res_tac parse_clause_aux_bound>>
+  fs[EVERY_REVERSE]
+QED
+
+(* Printing a parsed clause back *)
+val toStdString_def = Define`
+  toStdString i =
+    if 0i ≤ i ∧ i < 10 then
+      str (toChar (Num (ABS i)))
+    else
+      implode ((if i < 0i then "-" else "")++
+               (toChars (Num (ABS i) MOD maxSmall_DEC) (Num (ABS i) DIV maxSmall_DEC) ""))`;
+
+val print_clause_def = Define`
+  (print_clause [] = strlit "0\n") ∧
+  (print_clause (x::xs) =
+    toStdString x ^ strlit(" ") ^ print_clause xs)`
+
+Theorem tokens_unchanged:
+  EVERY ($~ o P) (explode ls) ∧ ¬ NULL (explode ls) ⇒
+  tokens P ls = [ls]
+Proof
+  rw[] >> drule TOKENS_unchanged>>
+  simp[]>>
+  simp[GSYM mlstringTheory.TOKENS_eq_tokens]
+QED
+
+(* TODO: Copied from mlintTheory *)
+Theorem toStdString_thm:
+   toStdString i = implode ((if i < 0i then "-" else "") ++ num_to_dec_string (Num (ABS i)))
+Proof
+  rw[toStdString_def]
+  >- (`F` by intLib.COOPER_TAC)
+  >- (
+    rw[mlstringTheory.str_def]
+    \\ AP_TERM_TAC
+    \\ `Num (ABS i) < 10` by intLib.COOPER_TAC
+    \\ simp[toChar_HEX]
+    \\ simp[ASCIInumbersTheory.num_to_dec_string_def]
+    \\ simp[ASCIInumbersTheory.n2s_def]
+    \\ simp[Once numposrepTheory.n2l_def])
+  \\ (
+    AP_TERM_TAC \\ simp[]
+    \\ `0 < maxSmall_DEC` by EVAL_TAC
+    \\ simp[toChars_thm]
+    \\ qspec_then`maxSmall_DEC`mp_tac DIVISION
+    \\ simp[] )
+QED
+
+Theorem fromString_toStdString[simp]:
+   !i:int. fromString (toStdString i) = SOME i
+Proof
+  rw [toStdString_thm, mlstringTheory.implode_def]
+  \\ qmatch_goalsub_abbrev_tac `strlit sss`
+  \\ qspec_then `sss` mp_tac fromString_thm
+  THEN1
+   (reverse impl_tac THEN1
+     (fs [Abbr`sss`,toString_thm,ASCIInumbersTheory.toNum_toString]
+      \\ rw [] \\ last_x_assum mp_tac \\ intLib.COOPER_TAC)
+    \\ fs [Abbr `sss`,EVERY_isDigit_num_to_dec_string])
+  \\ `HD sss ≠ #"~" ∧ HD sss ≠ #"-" ∧ HD sss ≠ #"+"` by
+   (fs [Abbr `sss`]
+    \\ qspec_then `Num (ABS i)` mp_tac EVERY_isDigit_num_to_dec_string
+    \\ Cases_on `num_to_dec_string (Num (ABS i))`
+    \\ fs []
+    \\ CCONTR_TAC \\ fs [] \\ rveq  \\ fs [isDigit_def])
+  \\ fs [Abbr `sss`,EVERY_isDigit_num_to_dec_string]
+  \\ fs [toString_thm,ASCIInumbersTheory.toNum_toString]
+  \\ rw [] \\ last_x_assum mp_tac \\ intLib.COOPER_TAC
+QED
+
+Theorem tokens_blanks_toStdString:
+  tokens blanks (toStdString h) = [toStdString h]
+Proof
+  match_mp_tac tokens_unchanged>>
+  rw[toStdString_thm]
+  >- EVAL_TAC
+  >- (
+    `EVERY isDigit (num_to_dec_string(Num(ABS h)))` by fs[ASCIInumbersTheory.EVERY_isDigit_num_to_dec_string]>>
+    pop_assum mp_tac >> match_mp_tac MONO_EVERY>>
+    EVAL_TAC>>rw[])
+  >- (
+    `EVERY isDigit (num_to_dec_string(Num(ABS h)))` by fs[ASCIInumbersTheory.EVERY_isDigit_num_to_dec_string]>>
+    pop_assum mp_tac >> match_mp_tac MONO_EVERY>>
+    EVAL_TAC>>rw[])
+  >>
+  Cases_on`num_to_dec_string(Num(ABS h))`>>fs[]
+QED
+
+Theorem tokens_print_clause_nonempty:
+  ∀ys. tokens blanks (print_clause ys) ≠ []
+Proof
+  Induct>>fs[print_clause_def]
+  >-
+    EVAL_TAC
+  >>
+  `blanks #" " ∧ str #" " = strlit " "` by EVAL_TAC>>
+  drule mlstringTheory.tokens_append>>simp[]
+QED
+
+Theorem parse_clause_aux_print_clause:
+  ∀ys maxvar acc.
+  EVERY (λl. Num (ABS l) ≤ maxvar) ys ∧
+  wf_clause ys
+  ⇒
+  parse_clause_aux maxvar (tokens blanks (print_clause ys)) acc = SOME (REVERSE ys ++ acc)
+Proof
+  Induct>>rw[print_clause_def]
+  >-
+    EVAL_TAC
+  >>
+  `blanks #" " ∧ str #" " = strlit " "` by EVAL_TAC>>
+  drule mlstringTheory.tokens_append>>simp[]>>
+  disch_then kall_tac>>
+  simp[tokens_blanks_toStdString]>>
+  Cases_on`tokens blanks (print_clause ys)`
+  >-
+    fs[tokens_print_clause_nonempty]
+  >>
+  simp[parse_clause_aux_def]>>fs[wf_clause_def]
+QED
+
+Theorem parse_clause_print_clause:
+  ∀ys maxvar.
+  EVERY (λl. Num (ABS l) ≤ maxvar) ys ∧
+  wf_clause ys
+  ⇒
+  parse_clause maxvar (tokens blanks (print_clause ys)) = SOME ys
+Proof
+  rw[parse_clause_def]>>
+  drule parse_clause_aux_print_clause>>
+  disch_then drule>>
+  disch_then (qspec_then`[]` assume_tac)>>simp[]
 QED
 
 val parse_header_line_def = Define`
@@ -63,6 +222,35 @@ val parse_header_line_def = Define`
     else NONE
   | _ => NONE`
 
+val print_header_line_def = Define`
+  print_header_line v len =
+  strlit ("p cnf ") ^  toStdString (&v) ^ strlit(" ") ^ toStdString (&len) ^ strlit("\n")`
+
+Theorem parse_header_line_print_header_line:
+  parse_header_line (tokens blanks (print_header_line v len)) = SOME(v,len)
+Proof
+  rw[print_header_line_def]>>
+  qmatch_goalsub_abbrev_tac`aa ^ bb ^ _ ^ cc ^ dd`>>
+  `blanks #" " ∧ str #" " = strlit " "` by EVAL_TAC>>
+  drule mlstringTheory.tokens_append>>simp[]>>
+  `aa = strlit"p" ^ strlit" " ^ strlit"cnf" ^ strlit" "` by
+    (fs[Abbr`aa`]>>EVAL_TAC)>>
+  strip_tac>>
+  first_assum(qspecl_then[`aa ^ bb`,`cc ^ dd`] assume_tac)>>fs[]>>
+  `cc ^ dd = cc ^ dd ^ strlit""` by EVAL_TAC>>
+  pop_assum SUBST_ALL_TAC>>
+  `blanks #"\n" ∧ str #"\n" = strlit "\n"` by EVAL_TAC>>
+  drule mlstringTheory.tokens_append>>simp[]>>
+  unabbrev_all_tac>>
+  simp[tokens_blanks_toStdString]>>
+  rw[]>>
+  `tokens blanks (strlit "p") = [strlit "p"]` by EVAL_TAC>>
+  `tokens blanks (strlit "cnf") = [strlit "cnf"]` by EVAL_TAC>>
+  `tokens blanks (strlit "") = []` by EVAL_TAC>>
+  simp[parse_header_line_def]>>
+  fs [num_to_str_def,fromNatString_def]
+QED
+
 (*
   parse strings as DIMACS
   For the DIMACS file, the *entire* file is read at once
@@ -70,7 +258,7 @@ val parse_header_line_def = Define`
 val build_fml_def = Define`
   (build_fml maxvar (id:num) [] (acc:ccnf) = SOME acc) ∧
   (build_fml maxvar id (s::ss) acc =
-    case parse_clause maxvar s [] of
+    case parse_clause maxvar s of
     NONE => NONE
   | SOME cl => build_fml maxvar (id+1) ss (insert id cl acc))`
 
@@ -97,7 +285,7 @@ Proof
   Induct>>rw[build_fml_def]>>fs[]>>
   every_case_tac>>fs[]>>
   imp_res_tac parse_clause_wf_clause>>fs[]>>
-  metis_tac[wf_fml_insert,parse_clause_wf_clause,wf_clause_def]
+  metis_tac[wf_fml_insert,parse_clause_wf_clause,wf_clause_def,MEM_REVERSE]
 QED
 
 Theorem build_fml_bound:
@@ -137,6 +325,153 @@ Proof
     qexists_tac`b`>>
     qexists_tac`d`>>
     unabbrev_all_tac>>fs[wf_fml_def,values_def,lookup_def]
+QED
+
+val max_lit_def = Define`
+  (max_lit k [] = k) ∧
+  (max_lit k (x::xs) = if k < ABS x then max_lit (ABS x) xs else max_lit k xs)`
+
+(* print a formula out to DIMACS *)
+val print_dimacs_def = Define`
+  print_dimacs fml =
+  let ls = MAP SND (toSortedAList fml) in
+  let len = LENGTH ls in
+  let v = max_lit 0 (MAP (max_lit 0) ls) in
+  print_header_line (Num v) len ::
+  MAP print_clause ls`
+
+Theorem FILTER_print_clause:
+  FILTER (λs. case s of x::xs => x ≠ strlit "c" | [] => T)
+    (MAP (tokens blanks) (MAP print_clause ls)) =
+    (MAP (tokens blanks) (MAP print_clause ls))
+Proof
+  simp[FILTER_EQ_ID,EVERY_MAP,EVERY_MEM]>>
+  rw[]>>
+  Cases_on`x`>>simp[print_clause_def]
+  >- EVAL_TAC >>
+  `blanks #" " ∧ str #" " = strlit " "` by EVAL_TAC>>
+  drule mlstringTheory.tokens_append>>simp[]>>
+  simp[tokens_blanks_toStdString,toStdString_thm]>>
+  rw[]>>
+  CCONTR_TAC>>fs[]>>
+  pop_assum (fn th => mp_tac (Q.AP_TERM `explode` th))>>
+  PURE_REWRITE_TAC [mlstringTheory.explode_implode]
+  >- simp[] >>
+  strip_tac>>
+  fs[]>>
+  `EVERY isDigit (toString (Num (ABS h)))` by
+    fs[EVERY_isDigit_num_to_dec_string]>>
+   rfs[]>>pop_assum mp_tac>>
+   EVAL_TAC
+QED
+
+Theorem build_fml_MAP_print_clause:
+  ∀vs id acc.
+  EVERY (λc. EVERY (λl. Num (ABS l) ≤ mv) c) vs ∧
+  EVERY wf_clause vs ∧
+  (∀x. x ∈ domain acc ⇒ x < id)
+  ⇒
+  ∃acc'.
+  build_fml mv id (MAP (tokens blanks) (MAP print_clause vs)) acc = SOME acc' ∧
+  values acc' = values acc ∪ set vs
+Proof
+  Induct>>rw[build_fml_def]>>
+  drule parse_clause_print_clause>> rw[]>>
+  fs[]>>
+  first_x_assum(qspecl_then[`id+1`,`insert id h acc`] mp_tac)>>
+  impl_tac>- (
+    rw[domain_insert]>>
+    fs[]>>
+    first_x_assum drule>>fs[])>>
+  rw[]>>
+  simp[]>>
+  simp[values_def,lookup_insert,EXTENSION]>>
+  rw[EQ_IMP_THM]>>pop_assum mp_tac>>rw[]
+  >- metis_tac[]
+  >- (
+    `n ∈ domain acc` by metis_tac[domain_lookup]>>
+    first_x_assum drule>>fs[]>>
+    strip_tac>>DISJ1_TAC>>qexists_tac`n`>>
+    fs[])
+  >- metis_tac[]
+QED
+
+Theorem print_header_line_first:
+  ∃ls. tokens blanks (print_header_line a b) =
+  strlit"p"::ls
+Proof
+  rw[print_header_line_def]>>
+  qmatch_goalsub_abbrev_tac`aa ^ bb ^ _ ^ dd ^ ee`>>
+  `aa = strlit"p" ^ strlit" " ^ strlit"cnf" ^ strlit" "` by
+    (fs[Abbr`aa`]>>EVAL_TAC)>>
+  simp[]>>
+  PURE_REWRITE_TAC[GSYM mlstringTheory.strcat_assoc]>>
+  PURE_REWRITE_TAC[Once mlstringTheory.strcat_assoc]>>
+  `blanks #" " ∧ str #" " = strlit " "` by EVAL_TAC>>
+  drule mlstringTheory.tokens_append>>simp[]>>
+  `tokens blanks (strlit "p") = [strlit "p"]` by EVAL_TAC>>
+  simp[]
+QED
+
+Theorem max_lit_max_1:
+  ∀ls k.
+  0 ≤ k ⇒
+  k ≤ max_lit k ls ∧
+  (∀x. MEM x ls ⇒ ABS x ≤ max_lit k ls)
+Proof
+  Induct>>rw[max_lit_def]>>
+  qmatch_goalsub_abbrev_tac`max_lit aa`>>
+  first_x_assum(qspec_then`aa` mp_tac)>>
+  simp[Abbr`aa`]>>
+  rw[] >>
+  intLib.COOPER_TAC
+QED
+
+Theorem max_lit_max:
+  (∀x. MEM x ls ⇒ ABS x ≤ max_lit 0 ls)
+Proof
+  `0 ≤ 0:int` by fs[]>>
+  metis_tac[max_lit_max_1]
+QED
+
+Theorem max_lit_max_lit_max:
+  EVERY (λc. EVERY (λl. Num (ABS l) ≤ Num (max_lit 0 (MAP (max_lit 0) vs))) c) vs
+Proof
+  rw[EVERY_MEM]>>
+  drule max_lit_max>>
+  strip_tac>>
+  `MEM (max_lit 0 c) (MAP (max_lit 0) vs)` by
+    (fs[MEM_MAP]>>metis_tac[])>>
+  drule max_lit_max>>
+  rw[]>>
+  intLib.ARITH_TAC
+QED
+
+Theorem parse_dimacs_print_dimacs:
+  wf_fml fml ⇒
+  ∃mv fml'.
+  parse_dimacs (print_dimacs fml) = SOME (mv, fml') ∧
+  values fml = values fml'
+Proof
+  simp[parse_dimacs_def,print_dimacs_def]>>
+  qmatch_goalsub_abbrev_tac`print_header_line a b`>>
+  assume_tac print_header_line_first>>fs[]>>
+  pop_assum sym_sub_tac>>
+  simp[parse_header_line_print_header_line]>>
+  unabbrev_all_tac>>
+  simp[FILTER_print_clause]>>
+  qmatch_goalsub_abbrev_tac`build_fml mv id (_ _ ( _ _ vs))`>>
+  strip_tac>>
+  qspecl_then [`vs`,`id`,`LN`] mp_tac build_fml_MAP_print_clause>>
+  impl_tac >- (
+    simp[]>>
+    CONJ_TAC >-
+      fs[Abbr`mv`,max_lit_max_lit_max]>>
+    fs[Abbr`vs`,EVERY_MAP,EVERY_MEM,wf_fml_def,values_def,FORALL_PROD,MEM_toSortedAList]>>
+    metis_tac[])>>
+  rw[]>>
+  simp[]>>
+  fs[lookup_def,values_def,Abbr`vs`,EXTENSION,MEM_MAP,EXISTS_PROD,MEM_toSortedAList]
 QED
 
 (* Parse a LPR clause with witness *)
@@ -328,39 +663,6 @@ Proof
   drule parse_lprstep_wf>>
   simp[]
 QED
-
-val max_lit_def = Define`
-  (max_lit k [] = k) ∧
-  (max_lit k (x::xs) = if ABS x > k then max_lit (ABS x) xs else max_lit k xs)`
-
-(*
-val toString_def = Define`
-  toString i =
-    if 0i ≤ i ∧ i < 10 then
-      str (toChar (Num (ABS i)))
-    else
-      implode ((if i < 0i then "-" else "")++
-               (toChars (Num (ABS i) MOD maxSmall_DEC) (Num (ABS i) DIV maxSmall_DEC) ""))`;
-*)
-
-val print_line_def = Define`
-  (print_line [] = strlit "0\n") ∧
-  (print_line (x::xs) =
-    mlint$toString x ^ strlit(" ") ^ print_line xs)`
-
-(* print a formula out to DIMACS *)
-val print_dimacs_def = Define`
-  print_dimacs fml =
-  let ls = MAP SND (toSortedAList fml) in
-  let len = LENGTH ls in
-  let v = max_lit 0 (MAP (max_lit 0) ls) in
-  (strlit ("p cnf ") ^  mlint$toString v ^ strlit(" ") ^  mlint$toString (&len) ^ strlit("\n"))::
-  MAP print_line ls`
-
-(* TODO: something like this would be good to know
-Theorem parse_of_print:
-  parse_dimacs (print_dimacs fml) = SOME fml
-*)
 
 val dimacsraw = ``[
   strlit "c this is a comment";
